Trees.v
@@ -1,7 +1,4 @@
 From mathcomp Require Import ssreflect ssrnat seq.
-From MonadicEffect Require Import Hoare.
-
-Require Import Program.
 
 Inductive Tree (a : Set) :=
 | Leaf : a -> Tree a
@@ -35,27 +32,3 @@ Fixpoint flatten {a : Set} (t : Tree a) : list a :=
   | Leaf x => x :: nil
   | Node l r => flatten l ++ flatten r
   end.
-
-Program Fixpoint relabel {a : Set} (t : Tree a) :
-  HoareState nat
-             (@top nat)
-             (Tree nat) 
-             (fun i t f => f = i + size t /\ flatten t = seq i (size t)) :=
-  match t with
-  | Leaf x =>
-    n <- get ;;
-    put (n + 1) ;;
-    ret (Leaf n)
-  | Node l r =>
-    l' <- relabel l ;;
-    r' <- relabel r ;;
-    ret (Node l' r')
-  end.
-Next Obligation.
-  case (relabel a l >>= _) => /=.
-  case=> x' n [t1] [n2] [[H0 H1] H2].
-  case: H2 => t2 [n3] [[H3 H4] [H5 H6]].  
-  rewrite H6. split => /=.
-  - rewrite -H5 H3 H0 addnA //.
-  - rewrite H1 H4 seq_split H0 //.
-Defined.
