Dijkstra.v
@@ -1,0 +1,64 @@
+From mathcomp Require Import ssreflect ssrnat.
+From MonadicEffect Require Import Trees.
+
+Require Import Program.
+
+Section Dijkstra.
+
+  Variables S : Set.
+
+  Definition WP {A} : Type := (A -> S -> Prop) -> S -> Prop.
+
+  Program Definition DST A (wp : WP) :=
+    forall p, { s : S | wp p s } -> { (a, s') : A * S | p a s' }.
+
+  Program Definition ret { A } (a : A) :
+    DST A (fun p => p a) :=
+    fun _ s => (a, s).
+
+  Program Definition bind : forall A wp1 B wp2,
+      DST A wp1 -> (forall a : A, DST B (wp2 a)) ->
+      DST B (fun p => wp1 (fun a => wp2 a p)) :=
+    fun A wp1 B wp2 c1 c2 _ s1 =>
+      let: (a, s2) := c1 _ s1 in c2 a _ s2.
+  Next Obligation.
+    elim: c1 Heq_anonymous => a' H' /= Heq_anonymous.
+    subst; done.
+  Defined.
+
+  Program Definition get : DST S (fun p s => p s s) :=
+    fun _ s => (s, s).
+
+  Program Definition put : forall s, DST unit (fun p _ => p tt s) :=
+    fun s _ _ => (tt, s).
+End Dijkstra.
+
+Arguments ret {S} {A}.
+Arguments bind {S} {A} {wp1} {B} {wp2}.
+Arguments get {S}.
+Arguments put {S}.
+
+Notation "c >>= f" := (bind c f) (at level 50, left associativity).
+Notation "f =<< c" := (bind c f) (at level 51, right associativity).
+Notation "x <- c1 ;; c2" := (bind c1 (fun x => c2)) (at level 100, c1 at next level, right associativity).
+Notation "e1 ;; e2" := (_ <- e1 ;; e2) (at level 100, right associativity).
+
+Program Fixpoint relabel {A : Set} (t : Tree A) :
+  DST nat (Tree nat) (fun p i =>
+                    forall t f, f = i + size t /\ flatten t = seq i (size t) ->
+                    p t f ) :=
+  match t with
+  | Leaf x =>
+    n <- get ;;
+    put (n + 1) ;;
+    ret (Leaf n)
+  | Node l r =>
+    l' <- relabel l ;;
+    r' <- relabel r ;;
+    ret (Node l' r')
+  end.
+Next Obligation.
+  apply H3. split => /=.
+  - by rewrite addnA.
+  - by rewrite H2 H1 seq_split.
+Defined.
